Lynx/Modules/Erlang/Definitions.lean
@@ -8,42 +8,42 @@ namespace Lynx.Modules.Erlang
 
 open Lynx
 
-def is_integer : Term → Result
+def is_integer_1 : Term → Result
   | .integer _ => .ok Term.true
   | _ => .ok Term.false
 
-def is_list : Term → Result
+def is_list_1 : Term → Result
   | .nil => .ok Term.true
   | .cons _ _ => .ok Term.true
   | _ => .ok Term.false
 
-def add : Term → Term → Result
+def add_2 : Term → Term → Result
   | .integer x, .integer y => .ok (.integer (x + y))
   | _, _ => throw (.error (.atom "badarith"))
 
-def equal (left right : Term) : Result :=
+def equal_2 (left right : Term) : Result :=
   .ok (if left = right then Term.true else Term.false)
 
-def less_than (left right : Term) : Result :=
+def less_than_2 (left right : Term) : Result :=
   .ok (if (Term.compare left right).isLT then Term.true else Term.false)
 
-def greater_than (left right : Term) : Result :=
+def greater_than_2 (left right : Term) : Result :=
   .ok (if (Term.compare left right).isGT then Term.true else Term.false)
 
-def less_than_or_equal (left right : Term) : Result :=
+def less_than_or_equal_2 (left right : Term) : Result :=
   .ok (if (Term.compare left right).isLE then Term.true else Term.false)
 
-def greater_than_or_equal (left right : Term) : Result :=
+def greater_than_or_equal_2 (left right : Term) : Result :=
   .ok (if (Term.compare left right).isGE then Term.true else Term.false)
 
-@[lynx_opaque] def append : Term → Term → Result
+@[lynx_opaque] def append_2 : Term → Term → Result
   | .nil, right => .ok right
   | .cons head tail, right => do
-      let rest ← append tail right
+      let rest ← append_2 tail right
       .ok (.cons head rest)
   | _, _ => throw (.error (.atom "badarg"))
 
-def andalso
+def andalso_2
     (left : Result)
     (right : Unit → Result) : Result :=
   match left with
